Complete presheaf model. A little progress in the report

Modèles/CWFU_presheaf.v
@@ -30,6 +30,14 @@ Definition fext {A B} {f g : forall x : A, B x} := functional_extensionality_dep
 
 Axiom UIP: forall {X} {x y:X} (p q :x = y) , p = q.
 
+Lemma rew_UIP {X} P {x} (y : P x) (H : x = x :> X) : rew [P] H in y = y.
+Proof.
+  change (rew [P] H in y = rew [P] eq_refl in y).
+  apply f_equal.
+  apply UIP. Show Proof.
+Defined.
+
+
 Record CWFU := {
   ctx : Type;
   typ : ctx -> Type;
@@ -186,8 +194,8 @@ Record psh_ctx := {
 
   ctx_id : forall {X} {x: ctx_obj X},
     ctx_fun cat_id x = x;
-  ctx_com : forall {X Y Z} {f: X ~> Y} {g: Y ~> Z} {z},
-    ctx_fun (cat_com g f) z = ctx_fun f (ctx_fun g z);
+  ctx_com : forall {X Y Z} {f: Y ~> Z} {g: X ~> Y} {z},
+    ctx_fun (cat_com f g) z = ctx_fun g (ctx_fun f z);
   } as Γ.
 Arguments ctx_id {Γ X x}.
 Arguments ctx_com {Γ X Y Z f g z}.
@@ -458,6 +466,46 @@ Proof.
   apply (ctx_obj (A_obj X x) X).
 Admitted. *)
 
+Record psh_app_obj {Γ} (A : ⊣ Γ) (X : cat_obj CC) : Type := mk_app
+  { app_tl : ctx_obj Γ X;
+    app_hd : typ_obj A app_tl }.
+
+Arguments mk_app {Γ A X}.
+Arguments app_tl {Γ A X}.
+Arguments app_hd {Γ A X}.
+
+Definition psh_app_fun {Γ} (A: ⊣ Γ) {X Y} (f: X ~> Y):
+  psh_app_obj A Y -> psh_app_obj A X := fun y => mk_app ((app_tl y)⋅f) ((app_hd y)⋅⋅ f).
+
+Lemma psh_app_obj_eq' {Γ} {A: ⊣ Γ} {X} {γ γ': ctx_obj Γ X} {a : typ_obj A γ} {a' : typ_obj A γ'}:
+  forall (H : γ = γ') (H': rew [typ_obj A] H in a = a'),
+  mk_app γ a = mk_app γ' a'.
+Proof.
+  intros <- <-.
+  reflexivity.
+Defined.
+Lemma psh_app_obj_eq {Γ} {A: ⊣ Γ} {X} {x x':psh_app_obj A X} : 
+  forall (H : app_tl x = app_tl x') (H': rew [typ_obj A] H in app_hd x = app_hd x'),
+  x = x'.
+Proof.
+  apply psh_app_obj_eq'.
+Defined.
+
+Definition psh_app Γ (A : ⊣ Γ) : ⊣.
+Proof.
+  refine {|
+    ctx_obj := psh_app_obj A;
+    ctx_fun X Y:= psh_app_fun A;
+    |}.
+  - intros X x.
+    apply psh_app_obj_eq with (H := ctx_id) (1:=typ_cat_id _).
+  - intros X Y Z f g z.
+    apply psh_app_obj_eq with (H := ctx_com) (1:= typ_cat_com _).
+Defined.
+
+Notation " Γ ⊳ A " := (psh_app Γ A) (at level 65).
+
+
 
 Record psh_sub (Γ Δ : psh_ctx) :={
   sub_obj : forall X:cat_obj CC, ctx_obj Γ X -> ctx_obj Δ X;
@@ -523,7 +571,7 @@ Defined.
 Notation "σ ∘ τ" := (psh_sub_com σ τ) (at level 65).
 
 
-Definition psh_neut_l {Γ Δ} : forall {σ: Γ ⊢ Δ},
+Definition psh_neu_l {Γ Δ} : forall {σ: Γ ⊢ Δ},
     psh_sub_com psh_sub_id σ = σ.
 Proof.
   intros σ.
@@ -532,7 +580,7 @@ Proof.
 Qed.
 
 
-Definition psh_neut_r {Γ Δ} : forall {σ:psh_sub Γ Δ},
+Definition psh_neu_r {Γ Δ} : forall {σ:psh_sub Γ Δ},
     psh_sub_com σ psh_sub_id = σ.
 Proof.
   intros σ.
@@ -653,9 +701,7 @@ Proof.
   intros X x.
   etransitivity.
   apply rew_trm. simpl. unfold psh_sub_trm_obj. simpl.
-  change (rew [fun var => var X x] f_equal typ_obj psh_typ_id in trm_obj t x = rew [fun var => var X x] eq_refl in trm_obj t x).
-  apply f_equal.
-  apply UIP.
+  apply (rew_UIP (fun var => var X x)).
 Qed.
 
 
@@ -668,12 +714,321 @@ Proof.
   etransitivity.
   apply rew_trm.
   simpl. unfold psh_sub_trm_obj. simpl. unfold psh_sub_com_obj.
-  change (rew [fun var => var X x] f_equal typ_obj psh_typ_com in trm_obj t (sub_obj τ (sub_obj σ x)) = rew [fun var => var X x] eq_refl in trm_obj t (sub_obj τ (sub_obj σ x))).
-  apply f_equal.
-  apply UIP.
+  apply (rew_UIP (fun var :forall X, ctx_obj Γ X -> Type => var X x) (trm_obj t (sub_obj τ (sub_obj σ x))) (f_equal typ_obj psh_typ_com)).
+Qed.
+
+Definition psh_wk_obj {Γ Δ} {A: ⊣ Γ} (σ : Γ ⊢ Δ) :  forall X (x: ctx_obj (Γ ⊳ A) X), ctx_obj Δ X:=
+  fun X x => sub_obj σ (app_tl x).
+Definition psh_wk {Γ Δ} (A: ⊣ Γ) (σ : Γ ⊢ Δ) : (Γ ⊳ A) ⊢ Δ.
+Proof.
+  refine {| sub_obj := psh_wk_obj σ|}.
+  intros X Y f y.
+  apply (sub_fun σ).
+Defined.
+
+Notation " σ • " := (psh_wk _ σ) (at level 65).
+
+
+Definition psh_wk_com {Γ Δ Ξ} : forall {σ: Γ ⊢ Δ} {τ: Δ ⊢ Ξ} {A: ⊣ Γ},
+  ((σ ∘ τ) • : Γ ⊳ A ⊢ Ξ ) = ((σ •) ∘ τ ).
+Proof.
+  intros σ τ A.
+  apply psh_sub_eq.
+  intros X x.
+  reflexivity.
+Qed.
+
+Definition psh_ext_obj {Γ Δ} {A: ⊣ Δ} (σ : Γ ⊢ Δ) (t : (A [σ]) ⊣ Γ):
+  forall X, ctx_obj Γ X -> ctx_obj (Δ ⊳ A) X :=
+  fun X x => (mk_app (sub_obj σ x) (trm_obj t x)).
+
+Definition psh_ext {Γ Δ} {A: ⊣ Δ} (σ : Γ ⊢ Δ) (t : (A [σ]) ⊣ Γ) :
+  Γ ⊢ (Δ ⊳ A).
+Proof.
+  refine {| sub_obj := psh_ext_obj σ t|}.
+  intros X Y f y.
+  apply psh_app_obj_eq with (H:= sub_fun σ f y).
+  simpl.
+  etransitivity.
+  apply (f_equal (fun var => rew _ in var)).
+  symmetry.
+  apply (trm_fun t). simpl. unfold psh_sub_typ_fun.
+  etransitivity.
+  apply rew_compose.
+  apply rew_UIP.
+Defined.
+
+Notation "σ ▸ t" := (psh_ext σ t) (at level 65).
+
+Definition psh_lst_obj {Γ} {A : ⊣ Γ} : forall X (x:ctx_obj (Γ ⊳ A) X),
+  typ_obj (psh_sub_typ A (psh_sub_id •)) x :=
+  fun X x => app_hd x.
+Definition psh_lst {Γ} {A : ⊣ Γ} :
+  (A [psh_sub_id •]) ⊣ (Γ ⊳ A) := {|trm_obj:=psh_lst_obj; trm_fun X Y f y:= eq_refl|}.
+
+
+Definition psh_wk_ext {Γ Δ Ξ} {A} {σ : Γ ⊢ Δ} {τ: Δ ⊢ Ξ} {t:A [σ] ⊣ Γ} :
+  (σ ▸ t) ∘ (τ •) = σ ∘ τ.
+Proof.
+  apply psh_sub_eq.
+  intros X x.
+  reflexivity.
 Qed.
 
 
+Definition psh_lst_ext {Γ Δ} A (σ: Γ ⊢ Δ) (t : (A [σ])⊣ Γ) :
+  rew [_] psh_neu_r in rew [fun X => (A [X]) ⊣ Γ] psh_wk_ext in rew <- [psh_trm Γ]  psh_typ_com in (psh_sub_trm psh_lst (σ ▸ t)) = t.
+Proof.
+  etransitivity. Print rew_compose.
+  apply (rew_compose (fun var => (A [var])⊣ Γ)).
+  etransitivity.
+  apply rew_map.
+  etransitivity.
+  apply rew_compose.
+  apply psh_trm_eq.
+  intros X x.
+  etransitivity.
+  apply rew_trm.
+  apply (rew_UIP (fun var => var X x)).
+Qed.
+
+Definition psh_ext_com {Γ Δ Ξ} {σ : Γ ⊢ Δ} {τ : Δ ⊢ Ξ} {A} {t : (A [τ]) ⊣ Δ}:
+  σ ∘ (τ ▸ t) = (σ ∘ τ) ▸ (rew <- [fun var => psh_trm Γ var] psh_typ_com in (t [: σ])).
+Proof.
+  apply psh_sub_eq.
+  intros X x. simpl. unfold psh_ext_obj.
+  apply (psh_app_obj_eq' (eq_refl)).
+  etransitivity.
+  2: apply (map_subst (fun var var' => @trm_obj Γ var var' X x) (eq_sym psh_typ_com)).
+  symmetry.
+  etransitivity.
+  apply (rew_map (fun var => var X x) (fun var : ⊣ Γ => @typ_obj Γ var) (eq_sym psh_typ_com)).
+  apply (rew_UIP (fun var => var X x) (trm_obj t (sub_obj σ x)) (f_equal (fun var => @typ_obj _ var) (eq_sym psh_typ_com))).
+Defined.
+
+Definition psh_wk_lst {Γ} {A : ⊣ Γ} : (psh_wk A psh_sub_id) ▸ psh_lst = psh_sub_id.
+Proof.
+  apply psh_sub_eq.
+  intros X x.
+  reflexivity.
+Defined.
+
+
+Definition psh_lft {Γ Δ} (A : ⊣ Δ) (σ : Γ ⊢ Δ) :
+  (Γ ⊳  (A [σ])) ⊢ (Δ ⊳ A) := (σ •) ▸ 
+  (rew [fun X => (_ [X •]) ⊣ _ ] psh_neu_l in
+  rew <- [fun X => (_ [X]) ⊣ _] psh_wk_com in
+  rew <- [fun X => X ⊣ _ ] psh_typ_com in
+  psh_lst (A:= A [σ])).
+
+Definition psh_lft_def : forall {Γ Δ} (A : ⊣ Δ) (σ : Γ ⊢ Δ),
+  psh_lft A σ = (σ •) ▸ 
+  (rew [fun X => (_ [X •]) ⊣ _ ] psh_neu_l in
+  rew <- [fun X => (_ [X]) ⊣ _] psh_wk_com in
+  rew <- [fun X => X ⊣ _ ] psh_typ_com in
+  psh_lst (A:= A [σ])).
+Proof. reflexivity. Qed.
+
+Definition psh_lft_ext {Γ Δ} {σ : Γ ⊢ Δ} {A : ⊣ Δ} {a : ( A [σ]) ⊣ Γ} : 
+     (psh_sub_id ▸ ( a [: psh_sub_id])) ∘ (psh_lft A σ) = σ ▸ a.
+Proof.
+  apply psh_sub_eq.
+  intros X x.
+  apply (psh_app_obj_eq' eq_refl).
+  simpl. etransitivity.
+  apply (f_equal (fun var: A[σ •] ⊣ (Γ ⊳ (A[σ])) => @trm_obj _ _ var X (psh_ext_obj psh_sub_id (a [:psh_sub_id]) X x))).
+  etransitivity.
+  apply (rew_map (fun var => (A [var]) ⊣ (Γ ⊳ (A[σ]))) (fun var => var •)).
+  etransitivity.
+  apply (rew_compose (fun var => (A [var]) ⊣ (Γ ⊳ (A [σ])))).
+  etransitivity.
+  apply (rew_map (fun var => var ⊣ (Γ ⊳ (A[σ]))) (fun var => A[var])).
+  apply rew_compose.
+  etransitivity.
+  apply (rew_trm (Γ ⊳ (A[σ])) _ _ _ (psh_ext_obj psh_sub_id (a [:psh_sub_id]) X x) (eq_trans (eq_sym psh_typ_com)
+    (f_equal (fun var : (Γ ⊳ (A [σ])) ⊢ Δ => A [var]) (eq_trans (eq_sym psh_wk_com)
+    (f_equal (fun var : Γ ⊢ Δ => var •) psh_neu_l)))) psh_lst).
+  simpl. unfold psh_sub_trm_obj. simpl.
+  apply (rew_UIP (fun var: forall X, psh_app_obj (A[σ]) X -> Type => var X (psh_ext_obj psh_sub_id (a [:psh_sub_id]) X x)) (trm_obj a x)
+    (f_equal typ_obj (eq_trans (eq_sym psh_typ_com) (f_equal (fun var : (Γ ⊳ (A [σ])) ⊢ Δ => A [var])
+    (eq_trans (eq_sym psh_wk_com) (f_equal (fun var : Γ ⊢ Δ => var •) psh_neu_l)))))).
+Defined.
+
+Record psh_pi_obj {Γ} {A : ⊣ Γ} (B : ⊣ (Γ ⊳ A)) {Z} (z : ctx_obj Γ Z) : Type := mk_pi_obj
+  {
+    pi_obj_obj : forall Y (f: Y ~> Z) (a : typ_obj A (z ⋅ f)), typ_obj B (mk_app (z ⋅ f) a);
+    pi_obj_fun : forall X Y (f: Y ~> Z) (g: X ~> Y) (a : typ_obj A (z ⋅ f)),
+      (rew ctx_com in pi_obj_obj X (cat_com f g)) (a ⋅⋅ g) = (pi_obj_obj Y f a) ⋅⋅ g;
+  }.
+
+Arguments mk_pi_obj {Γ A} B {Z} z.
+Arguments pi_obj_obj {Γ A B Z z}.
+Arguments pi_obj_fun {Γ A} B {Z} z.
+
+Lemma psh_pi_obj_eq' {Γ} {A : ⊣ Γ} (B : ⊣ (Γ ⊳ A)) Z (z : ctx_obj Γ Z) Π_obj Π_obj' Π_fun Π_fun':
+  (forall Y f a, Π_obj Y f a = Π_obj' Y f a) -> mk_pi_obj B z Π_obj Π_fun = mk_pi_obj B z Π_obj' Π_fun'.
+Proof.
+  intros H.
+  assert (Π_obj = Π_obj') as <-.
+  apply fext. intros Y.
+  apply fext. intros f.
+  apply fext. intros a.
+  apply H.
+  apply f_equal.
+  apply fext. intros X.
+  apply fext. intros Y.
+  apply fext. intros f.
+  apply fext. intros g.
+  apply fext. intros a.
+  apply UIP.
+Defined.
+
+Definition psh_pi_fun_obj {Γ} {A : ⊣ Γ} {B : ⊣ (Γ ⊳ A) }:
+  forall {Y Z} (f: Y ~> Z) z, psh_pi_obj B z ->
+  forall X (g : X ~> Y) a, typ_obj B (mk_app ((z ⋅ f) ⋅ g) a).
+Proof.
+  intros Y Z f z Π X g.
+  rewrite <- ctx_com.
+  intros a.
+  apply (pi_obj_obj Π).
+Defined.
+
+
+
+Definition psh_pi_fun_fun {Γ} {A : ⊣ Γ} {B : ⊣ (Γ ⊳ A) }:
+  forall {Y Z} (f: Y ~> Z) z (Π:psh_pi_obj B z),
+  forall W X (g : X ~> Y) (h : W ~> X)
+  (a : typ_obj A ((z ⋅ f) ⋅ g)),
+  (rew ctx_com in psh_pi_fun_obj f z Π W (cat_com g h)) (a ⋅⋅ h) = (psh_pi_fun_obj f z Π X g a) ⋅⋅ h.
+Proof.
+  intros Y Z f z Π W X g h a.
+  unfold psh_pi_fun_obj.
+  etransitivity.
+  apply (f_equal (fun var : forall a' : typ_obj A (((z ⋅ f) ⋅ g) ⋅ h), typ_obj B (mk_app (((z ⋅ f) ⋅ g) ⋅ h) a') => var (a ⋅⋅ h))).
+  etransitivity.
+  apply (rew_compose (fun var => forall a, typ_obj B (mk_app var a))).
+  etransitivity.
+  apply f_equal.
+  apply (UIP _ (eq_trans (f_equal (fun var : W ~> Z => z ⋅ var) cat_ass)
+  (eq_trans ctx_com (f_equal (fun var : ctx_obj Γ X => var ⋅ h) ctx_com)))).
+  symmetry.
+  etransitivity.
+  2: apply (rew_compose (fun var => forall a, typ_obj B (mk_app var a))).
+  etransitivity.
+  2: apply (rew_compose (fun var => forall a, typ_obj B (mk_app var a))).
+  etransitivity.
+  2: apply (rew_map (fun var => forall a, typ_obj B (mk_app var a)) (fun var => var ⋅ h)).
+  1: apply (f_equal (fun var => rew [fun var' => forall a, typ_obj B (mk_app (var' ⋅ h) a) ] ctx_com in rew [fun var' => forall a, typ_obj B (mk_app var' a)] ctx_com in var)).
+  1: etransitivity.
+  2: apply (rew_map (fun var => forall a, typ_obj B (mk_app var a)) (fun var => z ⋅ var)).
+  1: symmetry.
+  1:apply (f_equal_dep (fun var => forall a, typ_obj B (mk_app (z ⋅ var) a)) (fun var => pi_obj_obj Π W var)).
+  revert a.
+  rewrite <- (ctx_com (z:=z) (f:=f) (g:=g)). simpl.
+  intros a.
+  apply pi_obj_fun.
+Defined.
+
+
+Definition psh_pi_fun {Γ} {A : ⊣ Γ} {B : ⊣ (Γ ⊳ A) }:
+  forall {Y Z} (f: Y ~> Z) z, psh_pi_obj B z -> psh_pi_obj B (z ⋅ f).
+Proof.
+  intros X Y f z Π.
+  refine {|pi_obj_obj := psh_pi_fun_obj f z Π;
+    pi_obj_fun := psh_pi_fun_fun f z Π|}.
+Defined.
+
+  Definition psh_pi {Γ}: forall {A : ⊣ Γ} (B : ⊣ (Γ ⊳ A)), ⊣ Γ.
+  Proof.
+    intros A B.
+    refine {|typ_obj X := psh_pi_obj B; typ_fun X Y:= psh_pi_fun|}.
+    + intros X x b.
+      apply psh_pi_obj_eq'.
+      intros Y f a.
+      apply (f_equal (fun var => var a)).
+      etransitivity. symmetry.
+      apply (map_subst (P:= psh_pi_obj B) (fun var var' => pi_obj_obj var' Y f)).
+      simpl.
+      etransitivity.
+      apply (rew_map (fun var => forall a, typ_obj B (mk_app var a)) (fun var => var ⋅ f)).
+      unfold psh_pi_fun_obj.
+      etransitivity. Print rew_compose.
+      apply (rew_compose (fun var => forall a, typ_obj B (mk_app var a))).
+      etransitivity.
+      apply f_equal. apply (UIP _ (f_equal (fun var => x ⋅ var) cat_neu_l)).
+      rewrite (cat_neu_l (f:=f)).
+      reflexivity.
+    + intros X Y Z f g z b.
+      apply psh_pi_obj_eq'.
+      intros W h a.
+      apply (f_equal (fun var => var a)).
+      etransitivity. symmetry.
+      apply (map_subst (P:= psh_pi_obj B) (fun var var' => pi_obj_obj var' W h)).
+      simpl.
+      etransitivity.
+      apply (rew_map (fun var => forall a, typ_obj B (mk_app var a)) (fun var => var ⋅ h)).
+      unfold psh_pi_fun_obj.
+      etransitivity.
+      apply (rew_compose (fun var => forall a, typ_obj B (mk_app var a))).
+      etransitivity.
+      2: apply f_equal. Search (eq_sym (eq_sym _)).
+      2: apply eq_sym_involutive.
+      apply (rew_swap (fun var => forall a, typ_obj B (mk_app var a))).
+      etransitivity.
+      apply (rew_compose (fun var => forall a, typ_obj B (mk_app var a))).
+      etransitivity.
+      apply f_equal. Unshelve.
+     intros C D E f g e [b n].
+      unfold pshf_pi_fun. simpl.
+      unfold pshf_pi_fun_obj.
+      apply pshf_pi_obj_eq.
+      intros C' h a.
+      simpl.
+      rewrite <- (map_subst (P:= pshf_pi_obj B C)) with (f:= fun (y:pshf_obj Γ C) e => pi_obj e h).
+      simpl.
+      rewrite rew_map with (P:= fun p : pshf_obj Γ C' => forall a0 : A_obj A p, A_obj B {| app_c := p; app_a := a0 |})(f:=pshf_fun Γ h) (H:= pshf_comp).
+      repeat rewrite rew_compose.
+      let p := (match goal with [|- (rew [_] ?p in _) a = _ ] => p end) in
+      set (H := p); clearbody H.
+      let p := (match goal with [|- _ = (rew [_] ?p in _) a ] => p end) in
+      set (H' := p); clearbody H'.
+      revert a H'. rewrite <- H. clear.
+      intros a H.
+      assert (f_equal (fun X => pshf_fun Γ X e) (cat_assoc CC h f g) = H) as <- by apply UIP.
+      simpl.
+      rewrite <- rew_map with (f:= (fun X : C' ~> E => pshf_fun Γ X e)).
+      rewrite cat_assoc.
+      simpl. reflexivity.
+  Defined.
+Definition 
+
+  pi : forall {Γ} {A} (B : typ (app Γ A)), typ Γ;
+  sub_pi : forall {Γ Δ} {σ : sub Γ Δ} {A : typ Δ} {B : typ (app Δ A)},
+    sub_typ (pi B) σ = pi (sub_typ B (lft σ));
+  ev : forall {Γ} {A} {B : typ (app Γ A)} (f : trm Γ (pi B)) (a : trm Γ A),
+    trm Γ (sub_typ B (ext sub_id (sub_trm a sub_id)));
+  sub_ev : forall {Γ Δ} {σ : sub Γ Δ} {A} {B : typ (app Δ A)} {f a},
+    rew [fun X => trm Γ (sub_typ B (ext X (sub_trm a X)))] neu_r in
+    rew <- [fun X => trm Γ (sub_typ B (ext _ X))] (rew_swap _ _ _ trm_com) in
+    rew [fun X => trm Γ (sub_typ B X)] ext_com in
+    rew <- [fun X => trm Γ X] typ_com in
+    sub_trm (ev f a) σ =
+    rew [fun X => trm Γ (sub_typ B X)] lft_ext in
+    rew <- [trm Γ] typ_com in ev (rew [trm Γ] sub_pi in sub_trm f σ) (sub_trm a σ) :>
+    trm Γ (sub_typ B (ext σ (sub_trm a σ)));
+  abs : forall {Γ} {A : typ Γ} {B : typ (app Γ A)} (t : trm (app Γ A) B),
+    trm Γ (pi B);
+  sub_abs : forall {Γ Δ} {σ : sub Γ Δ} {A : typ Δ} {B : typ (app Δ A)} {t : trm (app Δ A) B},
+    rew sub_pi in sub_trm (abs t) σ = abs (sub_trm t (lft σ));
+  abs_ev : forall {Γ} {A} {B : typ (app Γ A)} (t : trm (app Γ A) B) (a : trm Γ A),
+    ev (abs t) a = sub_trm t (ext sub_id (sub_trm a sub_id));
+  eta : forall {Γ} {A} {B : typ (app Γ A)} (f : trm Γ (pi B)),
+    f =
+    rew [fun X => trm Γ (pi X)] typ_id in
+    rew [fun X => trm Γ (pi (sub_typ B  X))] wk_lst in
+    rew [fun X => trm Γ (pi (sub_typ B  X))] lft_ext in
+    rew <- [fun X => trm Γ (pi X)] typ_com in
+    abs (ev (rew [fun X => trm _ X] sub_pi in sub_trm f (wk A sub_id)) lst);
 
 
 
